theories/prepost.v
@@ -1,3 +1,5 @@
+Require Export iris.algebra.cmra.
+Require Export iris.algebra.updates.
 Require Export refframe.module.
 Require Import refframe.trefines.
 Require Import refframe.link.
@@ -7,59 +9,211 @@ Require Import refframe.proof_techniques.
 
 Set Default Proof Using "Type".
 
+Section updates.
+  Context {A : cmra}.
+  Lemma cmra_update_included (x y : A) :
+    x ≼ y → y ~~> x.
+  Proof. move => [? ->]. apply cmra_update_op_l. Qed.
+End updates.
+
+Section total_updates.
+  Local Set Default Proof Using "Type*".
+  Context {A : cmra}.
+  Lemma cmra_update_valid (x y : A) :
+    x ~~> y → ✓ x → ✓ y.
+  Proof.
+    move => Hupd /cmra_valid_validN Hvalid.
+    apply /cmra_valid_validN => n.
+    by apply (Hupd n None).
+  Qed.
+End total_updates.
+
+Section included.
+  Context {A : cmra}.
+  Implicit Types (x y z : A).
+  Lemma cmra_included_op_l x y z : x ≼ y → x ≼ y ⋅ z.
+  Proof. intros ?. etrans; [done|]. apply cmra_included_l. Qed.
+  Lemma cmra_included_op_r x y z : x ≼ y → x ≼ z ⋅ y.
+  Proof. intros ?. etrans; [done|]. apply cmra_included_r. Qed.
+End included.
+
 (** * prepost *)
 Section prepost.
 Context {R : Type}.
+Context {A : cmra}.
 
 Inductive prepost : Type :=
 | pp_end (r : R)
 | pp_prop (P : Prop) (pp : prepost)
 | pp_quant {T} (pp : T → prepost)
+| pp_add (P : A) (pp : prepost)
+| pp_remove (P : A) (pp : prepost)
+(* | pp_update (pp : prepost) *)
 .
 
-Fixpoint pp_to_ex (pp : prepost) (Q : R → Prop) : Prop :=
+Fixpoint pp_to_ex (pp : prepost) (x : A) (Q : R → A → Prop) : Prop :=
   match pp with
-  | pp_end r => Q r
-  | pp_prop P pp' => P ∧ pp_to_ex pp' Q
-  | pp_quant pp' => ∃ x, pp_to_ex (pp' x) Q
+  | pp_end r => Q r x
+  | pp_prop P pp' => P ∧ pp_to_ex pp' x Q
+  | pp_quant pp' => ∃ y, pp_to_ex (pp' y) x Q
+  | pp_add P pp' => ✓ (P ⋅ x) ∧ pp_to_ex pp' (P ⋅ x) Q
+  (* We could also put and ≡ here but that makes it more annoying for
+  the users because they probably always want an update. *)
+  | pp_remove P pp' => ∃ y, x ~~> (P ⋅ y) ∧ pp_to_ex pp' y Q
+  (* | pp_update pp' => ∃ y, x ~~> y ∧ pp_to_ex pp' y Q *)
   end.
 
-Fixpoint pp_to_all (pp : prepost) (Q : R → Prop) : Prop :=
+Fixpoint pp_to_all (pp : prepost) (x : A) (Q : R → A → Prop) : Prop :=
   match pp with
-  | pp_end r => Q r
-  | pp_prop P pp' => P → pp_to_all pp' Q
-  | pp_quant pp' => ∀ x, pp_to_all (pp' x) Q
+  | pp_end r => Q r x
+  | pp_prop P pp' => P → pp_to_all pp' x Q
+  | pp_quant pp' => ∀ y, pp_to_all (pp' y) x Q
+  | pp_add P pp' => ✓ (P ⋅ x) → pp_to_all pp' (P ⋅ x) Q
+  | pp_remove P pp' => ∀ y, x ~~> P ⋅ y → pp_to_all pp' y Q
+  (* | pp_update pp' => ∀ y, x ~~> y → pp_to_all pp' y Q *)
   end.
 
-Lemma pp_to_ex_exists pp Q:
-  pp_to_ex pp Q ↔ ∃ r, Q r ∧ pp_to_ex pp (r =.).
-Proof. elim: pp => /=; naive_solver. Qed.
+Lemma pp_to_ex_exists pp Q x:
+  pp_to_ex pp x Q ↔ ∃ r y, Q r y ∧ pp_to_ex pp x (λ r' y', r' = r ∧ y' = y).
+Proof. elim: pp x => /=; naive_solver. Qed.
 
-Lemma pp_to_all_forall pp Q:
-  pp_to_all pp Q ↔ (∀ r, pp_to_ex pp (r =.) → Q r).
-Proof. elim: pp => /=; naive_solver. Qed.
-Lemma pp_to_all_forall_2 pp Q:
-  pp_to_all pp Q →
-  ∀ r, pp_to_ex pp (r =.) → Q r.
+Lemma pp_to_all_forall pp Q x:
+  pp_to_all pp x Q ↔ (∀ r y, pp_to_ex pp x (λ r' y', r' = r ∧ y' = y) → Q r y).
+Proof. elim: pp x => /=; naive_solver. Qed.
+Lemma pp_to_all_forall_2 pp Q x:
+  pp_to_all pp x Q →
+  ∀ r y, pp_to_ex pp x (λ r' y', r' = r ∧ y' = y) → Q r y.
 Proof. apply pp_to_all_forall. Qed.
 
-Lemma pp_to_all_mono pp (Q1 Q2 : _ → Prop):
-  pp_to_all pp Q1 →
-  (∀ r, Q1 r → Q2 r) →
-  pp_to_all pp Q2.
-Proof. elim: pp => /=; naive_solver. Qed.
+Lemma pp_to_all_mono pp (Q1 Q2 : _ → _ → Prop) x:
+  pp_to_all pp x Q1 →
+  (∀ r y, Q1 r y → Q2 r y) →
+  pp_to_all pp x Q2.
+Proof. elim: pp x => /=; naive_solver. Qed.
 
-Lemma pp_to_ex_mono pp (Q1 Q2 : _ → Prop):
-  pp_to_ex pp Q1 →
-  (∀ r, Q1 r → Q2 r) →
-  pp_to_ex pp Q2.
-Proof. elim: pp => /=; naive_solver. Qed.
+Lemma pp_to_ex_mono pp (Q1 Q2 : _ → _ → Prop) x:
+  pp_to_ex pp x Q1 →
+  (∀ r y, Q1 r y → Q2 r y) →
+  pp_to_ex pp x Q2.
+Proof. elim: pp x => /=; naive_solver. Qed.
 
-Lemma pp_to_all_ex pp Q1 Q2:
-  pp_to_all pp Q1 →
-  pp_to_ex pp Q2 →
-  ∃ r, Q1 r ∧ Q2 r.
+Lemma pp_to_all_ex pp Q1 Q2 x:
+  pp_to_all pp x Q1 →
+  pp_to_ex pp x Q2 →
+  ∃ y r, Q1 r y ∧ Q2 r y.
 Proof. move => /pp_to_all_forall ? /pp_to_ex_exists. naive_solver. Qed.
+
+Definition pp_res_equiv (Q : R → A → Prop) (r : R) (x : A) : Prop :=
+  ∀ x', ✓ x' → x' ≡ x → Q r x'.
+
+Lemma pp_to_ex_mono_res pp (Q : _ → _ → Prop) x x':
+  x' ≡ x →
+  ✓ x' →
+  pp_to_ex pp x (pp_res_equiv Q) →
+  pp_to_ex pp x' Q.
+Proof.
+  elim: pp x x' => /=.
+  - naive_solver.
+  - naive_solver.
+  - naive_solver.
+  - move => P pp IH x x' Hequiv Hvalid [??]. rewrite {1}Hequiv.
+    split; [done|]. by apply: IH; [rewrite Hequiv..|done].
+  - move => P pp IH x x' Hequiv Hvalid [?[??]]. eexists _.
+    rewrite Hequiv. split; [done|].  apply: IH; [..|done]; [done|].
+    apply: cmra_update_valid; [|done].
+    rewrite Hequiv. etrans; [done|].
+    apply cmra_update_op_r.
+Qed.
+
+Lemma pp_to_all_mono_res pp (Q : _ → _ → Prop) x x':
+  x' ≡ x →
+  ✓ x' →
+  pp_to_all pp x (pp_res_equiv Q) →
+  pp_to_all pp x' Q.
+Proof.
+  elim: pp x x' => /=.
+  - naive_solver.
+  - naive_solver.
+  - naive_solver.
+  - move => P pp IH x x' Hequiv Hvalid ?. rewrite {1}Hequiv => ?.
+    apply: IH; [..|naive_solver]; by rewrite Hequiv.
+  - move => P pp IH x x' Hequiv Hvalid Hpp ?. rewrite Hequiv => ?.
+    apply: IH; [reflexivity| |naive_solver].
+    apply: cmra_update_valid; [|done].
+    rewrite Hequiv. etrans; [done|].
+    apply cmra_update_op_r.
+Qed.
+
+(*
+Definition pp_res_upd (Q : R → A → Prop) (r : R) (x : A) : Prop :=
+  ∀ x', ✓ x' → x' ~~> x → Q r x'.
+
+Lemma pp_to_ex_mono_upd pp (Q : _ → _ → Prop) x x':
+  x' ~~> x →
+  ✓ x' →
+  pp_to_ex pp x (pp_res_upd Q) →
+  pp_to_ex pp x' Q.
+Proof.
+  elim: pp x x' => /=.
+  - naive_solver.
+  - naive_solver.
+  - naive_solver.
+  - move => P pp IH x x' Hupd Hvalid [?[?[??]]]. eexists _.
+    split_and!.
+    + etrans; [by apply cmra_update_op|]. done.
+    + done.
+    + apply: IH; [..|done]; done.
+  - move => P pp IH x x' Hupd Hvalid [?[??]]. eexists _.
+    split.
+    + by etrans.
+    + apply: IH; [..|done].
+      done.
+      admit.
+Admitted.
+
+Definition pp_res_upd' (Q : R → A → Prop) (r : R) (x : A) : Prop :=
+  ∀ x', ✓ x → x ~~> x' → Q r x'.
+
+Lemma pp_to_all_mono_upd pp (Q : _ → _ → Prop) x x':
+  x ~~> x' →
+  ✓ x →
+  pp_to_all pp x (pp_res_upd' Q) →
+  pp_to_all pp x' Q.
+Proof.
+  elim: pp x x' => /=.
+  - naive_solver.
+  - naive_solver.
+  - naive_solver.
+  - move => P pp IH x x' Hupd Hvalid Hpp ???.
+    apply: IH; [| |apply Hpp].
+    + reflexivity.
+    + done.
+    + etrans; [by apply cmra_update_op|]. done.
+    + done.
+  - move => P pp IH x x' Hupd Hvalid Hpp y Hup2.
+    apply: IH; [| |apply Hpp].
+    + reflexivity.
+    + admit.
+    + by etrans.
+Admitted.
+
+Lemma pp_to_all_valid pp (Q : _ → _ → Prop) x:
+  ✓ x →
+  pp_to_all pp x (λ r x', ✓ x' → Q r x') →
+  pp_to_all pp x Q.
+Proof.
+  elim: pp x => /=.
+  - naive_solver.
+  - naive_solver.
+  - naive_solver.
+  - move => P pp IH x Hvalid Hpp x' Hupd ?.
+    by apply: IH; [|apply Hpp].
+  - move => P pp IH x Hvalid Hpp x' Hupd.
+    apply: IH; [|apply Hpp].
+    + admit.
+    + done.
+Admitted.
+*)
 End prepost.
 
 Arguments prepost : clear implicits.
@@ -67,7 +221,8 @@ Arguments prepost : clear implicits.
 (** * mod_prepost *)
 Section prepost.
   Context {EV1 EV2 S : Type}.
-  Implicit Types (i : EV2 → S → prepost (EV1 * S)) (o : EV1 → S → prepost (EV2 * S)).
+  Context {A : cmra}.
+  Implicit Types (i : EV2 → S → prepost (EV1 * S) A) (o : EV1 → S → prepost (EV2 * S) A).
   Implicit Types (m : module EV1).
 
   Inductive pp_state : Type :=
@@ -80,20 +235,20 @@ Section prepost.
   .
 
   Inductive pp_filter_step i o :
-    (pp_state * S) → option (EV1 + EV2) → ((pp_state * S) → Prop) → Prop :=
-  | PPOutsideS s e:
-    pp_filter_step i o (PPOutside, s) (Some (inr e)) (λ σ, σ = (PPRecv1 e, s))
-  | PPRecv1S s e:
-    pp_filter_step i o (PPRecv1 e, s) None (λ σ, pp_to_ex (i e s) (λ r, σ = (PPRecv2 r.1, r.2)))
-  | PPRecv2S s e:
-    pp_filter_step i o (PPRecv2 e, s) (Some (inl e)) (λ σ, σ = (PPInside, s))
-  | PPInsideS s e:
-    pp_filter_step i o (PPInside, s) (Some (inl e)) (λ σ, σ = (PPSend1 e, s))
-  | PPSend1S s e r:
-    pp_to_ex (o e s) (r=.) →
-    pp_filter_step i o (PPSend1 e, s) None (λ σ, σ = (PPSend2 r.1, r.2))
-  | PPSend2S s e:
-    pp_filter_step i o (PPSend2 e, s) (Some (inr e)) (λ σ, σ = (PPOutside, s))
+    (pp_state * S * A) → option (EV1 + EV2) → ((pp_state * S * A) → Prop) → Prop :=
+  | PPOutsideS s x e:
+    pp_filter_step i o (PPOutside, s, x) (Some (inr e)) (λ σ, σ = (PPRecv1 e, s, x))
+  | PPRecv1S s x e:
+    pp_filter_step i o (PPRecv1 e, s, x) None (λ σ, pp_to_ex (i e s) x (λ r y, σ = (PPRecv2 r.1, r.2, y)))
+  | PPRecv2S s x e:
+    pp_filter_step i o (PPRecv2 e, s, x) (Some (inl e)) (λ σ, σ = (PPInside, s, x))
+  | PPInsideS s x e:
+    pp_filter_step i o (PPInside, s, x) (Some (inl e)) (λ σ, σ = (PPSend1 e, s, x))
+  | PPSend1S s x e r y:
+    pp_to_ex (o e s) x (λ r' y', r' = r ∧ y' = y) →
+    pp_filter_step i o (PPSend1 e, s, x) None (λ σ, σ = (PPSend2 r.1, r.2, y))
+  | PPSend2S s x e:
+    pp_filter_step i o (PPSend2 e, s, x) (Some (inr e)) (λ σ, σ = (PPOutside, s, x))
   .
 
   Definition mod_prepost_filter i o :=
@@ -115,18 +270,18 @@ Section prepost.
     move => ?. apply mod_seq_map_trefines => //. apply _.
   Qed.
 
-  Lemma mod_prepost_step_Outside_i i o m σ s:
-    TStepI (mod_prepost i o m) (SMFilter, σ, (PPOutside, s)) (λ G,
-        ∀ e, G true (Some e) (λ G', G' (SMFilter, σ, (PPRecv1 e, s)))).
+  Lemma mod_prepost_step_Outside_i i o m σ s x:
+    TStepI (mod_prepost i o m) (SMFilter, σ, (PPOutside, s, x)) (λ G,
+        ∀ e, G true (Some e) (λ G', G' (SMFilter, σ, (PPRecv1 e, s, x)))).
   Proof.
     constructor => G /= ?. tstep_i.
     apply steps_impl_step_end => ???. invert_all @m_step => ???. split! => ?. split!; [naive_solver|done|].
     naive_solver.
   Qed.
 
-  Lemma mod_prepost_step_Recv1_i i o m σ s e:
-    TStepI (mod_prepost i o m) (SMFilter, σ, (PPRecv1 e, s)) (λ G,
-        pp_to_ex (i e s) (λ r, G true None (λ G', G' (SMProgRecv r.1, σ, (PPInside, r.2))))).
+  Lemma mod_prepost_step_Recv1_i i o m σ s e x:
+    TStepI (mod_prepost i o m) (SMFilter, σ, (PPRecv1 e, s, x)) (λ G,
+        pp_to_ex (i e s) x (λ r y, G true None (λ G', G' (SMProgRecv r.1, σ, (PPInside, r.2, y))))).
   Proof.
     constructor => G /= /pp_to_ex_exists[r [HG Hex]]. tstep_i.
     apply steps_impl_step_next => ???. invert_all @m_step.
@@ -134,45 +289,45 @@ Section prepost.
     apply steps_impl_step_end => ???. invert_all @m_step => ???. naive_solver.
   Qed.
 
-  Lemma mod_prepost_step_Inside_i i o m σ s e:
-    TStepI (mod_prepost i o m) (SMFilterRecv e, σ, (PPInside, s)) (λ G,
-        pp_to_all (o e s) (λ r, G true (Some (r.1)) (λ G', G' (SMFilter, σ, (PPOutside, r.2))))).
+  Lemma mod_prepost_step_Inside_i i o m σ s e x:
+    TStepI (mod_prepost i o m) (SMFilterRecv e, σ, (PPInside, s, x)) (λ G,
+        pp_to_all (o e s) x (λ r y, G true (Some (r.1)) (λ G', G' (SMFilter, σ, (PPOutside, r.2, y))))).
   Proof.
     constructor => G /= ?. apply steps_impl_step_trans. tstep_i.
     apply steps_impl_step_end => ???. invert_all @m_step => ? b *; simplify_eq. split! => ?. split!; [done|].
     tstep_i.
     apply steps_impl_step_next => ???. invert_all @m_step => *; simplify_eq. split!.
     apply steps_impl_step_end => ???. invert_all @m_step => *; simplify_eq. split! => ?.
-    have [?[??]]:= pp_to_all_ex _ _ _ ltac:(done) ltac:(done); subst.
+    have [?[?[?[??]]]]:= pp_to_all_ex _ _ _ _ ltac:(done) ltac:(done); subst.
     split!; [done|by destruct b|]. naive_solver.
   Qed.
 
-  Lemma mod_prepost_step_Outside_s i o m σ s:
-    TStepS (mod_prepost i o m) (SMFilter, σ, (PPOutside, s)) (λ G,
-        ∃ e, G (Some e) (λ G', G' (SMFilter, σ, (PPRecv1 e, s)))).
+  Lemma mod_prepost_step_Outside_s i o m σ s x:
+    TStepS (mod_prepost i o m) (SMFilter, σ, (PPOutside, s, x)) (λ G,
+        ∃ e, G (Some e) (λ G', G' (SMFilter, σ, (PPRecv1 e, s, x)))).
   Proof.
     constructor => G /= [??]. split!; [done|] => /= ??. tstep_s. eexists (Some (inr _)). split!.
     apply: steps_spec_step_end; [by econs|]. naive_solver.
   Qed.
 
 
-  Lemma mod_prepost_step_Recv1_s i o m σ s e:
-    TStepS (mod_prepost i o m) (SMFilter, σ, (PPRecv1 e, s)) (λ G,
-        G None (λ G', pp_to_all (i e s) (λ r, G' (SMProgRecv r.1, σ, (PPInside, r.2))))).
+  Lemma mod_prepost_step_Recv1_s i o m σ s e x:
+    TStepS (mod_prepost i o m) (SMFilter, σ, (PPRecv1 e, s, x)) (λ G,
+        G None (λ G', pp_to_all (i e s) x (λ r y, G' (SMProgRecv r.1, σ, (PPInside, r.2, y))))).
   Proof.
     constructor => G /= ?. split!; [done|] => /= ??. apply steps_spec_step_trans.
     tstep_s. eexists None. split!.
     apply: steps_spec_step_end; [by econs|] => ? /=?.
-    have [?[??]]:= pp_to_all_ex _ _ _ ltac:(done) ltac:(done); subst.
+    have [?[?[??]]]:= pp_to_all_ex _ _ _ _ ltac:(done) ltac:(done); subst.
     tstep_s. eexists (Some (inl _)). split!.
     apply: steps_spec_step_end; [by econs|]. naive_solver.
   Qed.
 
-  Lemma mod_prepost_step_Inside_s i o m σ s e:
-    TStepS (mod_prepost i o m) (SMFilterRecv e, σ, (PPInside, s)) (λ G,
-        pp_to_ex (o e s) (λ r, G (Some (r.1)) (λ G', G' (SMFilter, σ, (PPOutside, r.2))))).
+  Lemma mod_prepost_step_Inside_s i o m σ s e x:
+    TStepS (mod_prepost i o m) (SMFilterRecv e, σ, (PPInside, s, x)) (λ G,
+        pp_to_ex (o e s) x (λ r y, G (Some (r.1)) (λ G', G' (SMFilter, σ, (PPOutside, r.2, y))))).
   Proof.
-    constructor => G /= /pp_to_ex_exists[?[??]]. split!; [done|] => /= ??.
+    constructor => G /= /pp_to_ex_exists[?[?[??]]]. split!; [done|] => /= ??.
     apply steps_spec_step_trans. tstep_s. eexists (Some _). split!.
     apply: steps_spec_step_end; [by econs|] => /= ? ->. tstep_s. eexists (Some (inr _)). split!.
     apply: steps_spec_step; [by econs|] => /= ? ->.
@@ -190,29 +345,29 @@ Global Hint Resolve
        mod_prepost_step_Inside_s
  | 3 : tstep.
 
-Definition prepost_id {EV} : EV → unit → prepost (EV * unit) :=
+Definition prepost_id {EV} : EV → unit → prepost (EV * unit) unitR :=
   λ x _, pp_end (x, tt).
 
-Lemma prepost_id_l S EV1 EV2 (m : module EV1) σ i o s:
+Lemma prepost_id_l A S EV1 EV2 (m : module EV1) σ i o s x:
   trefines (MS (mod_prepost i o (mod_prepost prepost_id prepost_id m))
-               (SMFilter, (SMFilter, σ, (PPOutside, tt)), (PPOutside, s)))
-           (MS (mod_prepost (S:=S) (EV2:=EV2) i o m) (SMFilter, σ, (PPOutside, s))).
+               (SMFilter, (SMFilter, σ, (PPOutside, tt, tt)), (PPOutside, s, x)))
+           (MS (mod_prepost (A:=A) (S:=S) (EV2:=EV2) i o m) (SMFilter, σ, (PPOutside, s, x))).
 Proof.
   apply tsim_implies_trefines => /= n.
   tstep_i => ?.
   tstep_s. split!.
-  tstep_s. apply pp_to_all_forall => ??.
+  tstep_s. apply pp_to_all_forall => ???.
   tstep_i. apply: pp_to_ex_mono; [done|].
-  move => ? <-.
+  move => ?? [<- <-].
   tstep_i => ? <-.
   tstep_i.
   unshelve apply: tsim_remember. { simpl. exact (λ _
-      '(σf1, (σf1', σ1, (σpp1', _)), (σpp1, s1)) '(σf2, σ2, (σpp2, s2)),
-         σf1 = SMProg ∧ σf1' = σf2 ∧ σ1 = σ2 ∧ σpp1 = PPInside
+      '(σf1, (σf1', σ1, (σpp1', _, _)), (σpp1, s1, x1)) '(σf2, σ2, (σpp2, s2, x2)),
+         σf1 = SMProg ∧ σf1' = σf2 ∧ σ1 = σ2 ∧ σpp1 = PPInside ∧ x1 = x2
          ∧ σpp1' = PPInside ∧ σpp2 = PPInside ∧ s1 = s2 ∧
          ((∃ e, σf1' = SMProgRecv e) ∨ σf1' = SMProg)). }
   { split!. } { done. }
-  move => {}n _ Hloop [[σf1 [[σf1' σ1] [σpp1' []]] [σpp1 s1]]] [[σf2 σ2] [σpp2 s2]] ?.
+  move => {}n _ Hloop [[σf1 [[σf1' σ1] [[σpp1' []] ?]] [[σpp1 s1] x1]]] [[σf2 σ2] [[σpp2 s2] x2]] ?.
   destruct_all?; simplify_eq.
   - tstep_both. apply: steps_impl_step_end => κ ??. case_match => *.
     + subst. tstep_s. eexists (Some _). split!.
@@ -223,12 +378,12 @@ Proof.
   - tstep_both. apply: steps_impl_step_end => κ ??.
     tstep_s. eexists _. apply: steps_spec_step_end; [done|] => ??.
     case_match; tend; (split!; [done|]). 2: { apply: Hloop; [done|]. split!. }
-    tstep_i. tstep_i. apply pp_to_all_forall => ??.
-    tstep_s. apply: pp_to_ex_mono; [done|]. move => ? <-. split!.
+    tstep_i. tstep_i. apply pp_to_all_forall => ???.
+    tstep_s. apply: pp_to_ex_mono; [done|]. move => ?? [<- <-]. split!.
     tstep_i => ?.
     tstep_s. split!.
-    tstep_s. apply pp_to_all_forall => ??.
-    tstep_i. apply: pp_to_ex_mono; [done|]. move => ? <-.
+    tstep_s. apply pp_to_all_forall => ???.
+    tstep_i. apply: pp_to_ex_mono; [done|]. move => ?? [<- <-].
     tstep_i => ? <-.
     tstep_i.
     apply Hloop; [done|]. split!.
@@ -245,139 +400,167 @@ Section prepost.
 
   Lemma mod_prepost_link
         {EV1 EV2 S1 S2 S' Sr1 Sr2 : Type}
-        (INV : seq_product_state → S1 → S2 → S' → Sr1 → Sr2 → Prop)
-        (i1 : io_event EV2 → S1 → prepost (io_event EV1 * S1))
-        (o1 : io_event EV1 → S1 → prepost (io_event EV2 * S1))
-        (i2 : io_event EV2 → S2 → prepost (io_event EV1 * S2))
-        (o2 : io_event EV1 → S2 → prepost (io_event EV2 * S2))
-        (i : io_event EV2 → S' → prepost (io_event EV1 * S'))
-        (o : io_event EV1 → S' → prepost (io_event EV2 * S'))
+        {A : cmra}
+        (INV : seq_product_state → S1 → S2 → S' → A → A → Sr1 → Sr2 → Prop)
+        (i1 : io_event EV2 → S1 → prepost (io_event EV1 * S1) A)
+        (o1 : io_event EV1 → S1 → prepost (io_event EV2 * S1) A)
+        (i2 : io_event EV2 → S2 → prepost (io_event EV1 * S2) A)
+        (o2 : io_event EV1 → S2 → prepost (io_event EV2 * S2) A)
+        (i : io_event EV2 → S' → prepost (io_event EV1 * S') A)
+        (o : io_event EV1 → S' → prepost (io_event EV2 * S') A)
         (R1 : seq_product_state → Sr1 → EV2 → seq_product_state → Sr1 → EV2 → Prop)
         (R2 : seq_product_state → Sr2 → EV1 → seq_product_state → Sr2 → EV1 → Prop)
         (m1 m2 : module (io_event EV1))
-        σ1 σ2 s1 s2 sr1 sr2 s
+        σ1 σ2 s1 s2 x1 x2 x sr1 sr2 s
         `{!VisNoAll m1} `{!VisNoAll m2}
         :
 
        (∀ p s e p' s' e', R1 p s e p' s' e' → p ≠ p') →
-       INV SPNone s1 s2 s sr1 sr2 →
-       (∀ s1 s2 s sr1 sr2 e sr1' e',
+       x ≡ x1 ⋅ x2 →
+       ✓ x →
+       INV SPNone s1 s2 s x1 x2 sr1 sr2 →
+       (∀ s1 s2 s x1 x2 sr1 sr2 e sr1' e',
+          INV SPNone s1 s2 s x1 x2 sr1 sr2 →
+          ✓ (x1 ⋅ x2) →
           R1 SPNone sr1 e SPLeft sr1' e' →
-          INV SPNone s1 s2 s sr1 sr2 →
-          pp_to_all (i (Incoming, e') s) (λ r1,
-          pp_to_ex (i1 (Incoming, e') s1) (λ r2, ∃ e sr2',
+          pp_to_all (i (Incoming, e') s) (x1 ⋅ x2) (λ r1 y1,
+          pp_to_ex (i1 (Incoming, e') s1) x1 (λ r2 y2, ∃ e sr2',
             r1.1.1 = Incoming ∧
             r2.1.1 = Incoming ∧
             r1.1.2 = r2.1.2 ∧
+            y1 ~~> y2 ⋅ x2 ∧
             R2 SPNone sr2 e SPLeft sr2' r1.1.2 ∧
-            INV SPLeft r2.2 s2 r1.2 sr1' sr2'))) →
-       (∀ s1 s2 s sr1 sr2 e sr1' e',
+            INV SPLeft r2.2 s2 r1.2 y2 x2 sr1' sr2'))) →
+       (∀ s1 s2 s x1 x2 sr1 sr2 e sr1' e',
+          INV SPNone s1 s2 s x1 x2 sr1 sr2 →
+          ✓ (x1 ⋅ x2) →
           R1 SPNone sr1 e SPRight sr1' e' →
-          INV SPNone s1 s2 s sr1 sr2 →
-          pp_to_all (i (Incoming, e') s) (λ r1,
-          pp_to_ex (i2 (Incoming, e') s2) (λ r2, ∃ e sr2',
+          pp_to_all (i (Incoming, e') s) (x1 ⋅ x2) (λ r1 y1,
+          pp_to_ex (i2 (Incoming, e') s2) x2 (λ r2 y2, ∃ e sr2',
             r1.1.1 = Incoming ∧
             r2.1.1 = Incoming ∧
             r1.1.2 = r2.1.2 ∧
+            y1 ~~> x1 ⋅ y2 ∧
             R2 SPNone sr2 e SPRight sr2' r1.1.2 ∧
-            INV SPRight s1 r2.2 r1.2 sr1' sr2'))) →
-       (∀ s1 s2 s sr1 sr2 e,
-           INV SPLeft s1 s2 s sr1 sr2 →
-           pp_to_all (o1 e s1) (λ r1, ∀ sr1' e',
+            INV SPRight s1 r2.2 r1.2 x1 y2 sr1' sr2'))) →
+       (∀ s1 s2 s x1 x2 sr1 sr2 e,
+           INV SPLeft s1 s2 s x1 x2 sr1 sr2 →
+           ✓ (x1 ⋅ x2) →
+           pp_to_all (o1 e s1) x1 (λ r1 y1, ∀ sr1' e',
              r1.1.1 = Outgoing →
              R1 SPLeft sr1 r1.1.2 SPRight sr1' e' →
-             pp_to_ex (i2 (Incoming, e') s2) (λ r2, ∃ sr2',
+             pp_to_ex (i2 (Incoming, e') s2) x2 (λ r2 y2, ∃ sr2',
                e.1 = Outgoing ∧
                r2.1.1 = Incoming ∧
-               INV SPRight r1.2 r2.2 s sr1' sr2' ∧
+               x1 ⋅ x2 ~~> y1 ⋅ y2 ∧
+               INV SPRight r1.2 r2.2 s y1 y2 sr1' sr2' ∧
                R2 SPLeft sr2 e.2 SPRight sr2' r2.1.2))) →
-       (∀ s1 s2 s sr1 sr2 e,
-           INV SPLeft s1 s2 s sr1 sr2 →
-           pp_to_all (o1 e s1) (λ r1, ∀ sr1' e',
+       (∀ s1 s2 s x1 x2 sr1 sr2 e,
+           INV SPLeft s1 s2 s x1 x2 sr1 sr2 →
+           ✓ (x1 ⋅ x2) →
+           ∀ x, x ~~> (x1 ⋅ x2) →
+           pp_to_all (o1 e s1) x1 (λ r1 y1, ∀ sr1' e',
              r1.1.1 = Outgoing →
              R1 SPLeft sr1 r1.1.2 SPNone sr1' e' →
              ∃ e'' sr2',
                e.1 = Outgoing ∧
                R2 SPLeft sr2 e.2 SPNone sr2' e'' ∧
-               pp_to_ex (o (Outgoing, e'') s) (λ r2,
+               pp_to_ex (o (Outgoing, e'') s) x (λ r2 y2,
                  r2.1.1 = Outgoing ∧
                  r2.1.2 = e' ∧
-                 INV SPNone r1.2 s2 r2.2 sr1' sr2'))) →
-       (∀ s1 s2 s sr1 sr2 e,
-           INV SPRight s1 s2 s sr1 sr2 →
-           pp_to_all (o2 e s2) (λ r1, ∀ sr1' e',
+                 (* This = instead of ≡ is fine because the pp_to_ex
+                 must have a update in it. *)
+                 y2 = y1 ⋅ x2 ∧
+                 INV SPNone r1.2 s2 r2.2 y1 x2 sr1' sr2'))) →
+       (∀ s1 s2 s x1 x2 sr1 sr2 e,
+           INV SPRight s1 s2 s x1 x2 sr1 sr2 →
+           ✓ (x1 ⋅ x2) →
+           pp_to_all (o2 e s2) x2 (λ r1 y1, ∀ sr1' e',
              r1.1.1 = Outgoing →
              R1 SPRight sr1 r1.1.2 SPLeft sr1' e' →
-             pp_to_ex (i1 (Incoming, e') s1) (λ r2, ∃ sr2',
+             pp_to_ex (i1 (Incoming, e') s1) x1 (λ r2 y2, ∃ sr2',
                e.1 = Outgoing ∧
                r2.1.1 = Incoming ∧
-               INV SPLeft r2.2 r1.2 s sr1' sr2' ∧
+               x1 ⋅ x2 ~~> y2 ⋅ y1 ∧
+               INV SPLeft r2.2 r1.2 s y2 y1 sr1' sr2' ∧
                R2 SPRight sr2 e.2 SPLeft sr2' r2.1.2))) →
-       (∀ s1 s2 s sr1 sr2 e,
-           INV SPRight s1 s2 s sr1 sr2 →
-           pp_to_all (o2 e s2) (λ r1, ∀ sr1' e',
+       (∀ s1 s2 s x1 x2 sr1 sr2 e,
+           INV SPRight s1 s2 s x1 x2 sr1 sr2 →
+           ✓ (x1 ⋅ x2) →
+           ∀ x, x ~~> (x1 ⋅ x2) →
+           pp_to_all (o2 e s2) x2 (λ r1 y1, ∀ sr1' e',
              r1.1.1 = Outgoing →
              R1 SPRight sr1 r1.1.2 SPNone sr1' e' →
              ∃ e'' sr2',
                e.1 = Outgoing ∧
                R2 SPRight sr2 e.2 SPNone sr2' e'' ∧
-               pp_to_ex (o (Outgoing, e'') s) (λ r2,
+               pp_to_ex (o (Outgoing, e'') s) x (λ r2 y2,
                  r2.1.1 = Outgoing ∧
                  r2.1.2 = e' ∧
-                 INV SPNone s1 r1.2 r2.2 sr1' sr2'))) →
+                 (* This = instead of ≡ is fine because the pp_to_ex
+                 must have a update in it. *)
+                 y2 = x1 ⋅ y1 ∧
+                 INV SPNone s1 r1.2 r2.2 x1 y1 sr1' sr2'))) →
     trefines (MS (mod_link R1 (mod_prepost i1 o1 m1) (mod_prepost i2 o2 m2))
-                 (MLFNone, sr1, (SMFilter, σ1, (PPOutside, s1)), (SMFilter, σ2, (PPOutside, s2))))
+                 (MLFNone, sr1, (SMFilter, σ1, (PPOutside, s1, x1)), (SMFilter, σ2, (PPOutside, s2, x2))))
              (MS (mod_prepost i o (mod_link R2 m1 m2))
-                 (SMFilter, (MLFNone, sr2, σ1, σ2), (PPOutside, s))).
+                 (SMFilter, (MLFNone, sr2, σ1, σ2), (PPOutside, s, x))).
     Proof.
-      move => Hneq Hinv HN2L HN2R HL2R HL2N HR2L HR2N.
+      move => Hneq Hequiv Hvalid Hinv HN2L HN2R HL2R HL2N HR2L HR2N.
       apply tsim_implies_trefines => /= n.
       unshelve apply: tsim_remember. { simpl. exact (λ _
-          '(σl1, sr1, (σf1, σ1, (σpp1, s1)), (σf2, σ2, (σpp2, s2)))
-          '(σf, (σl2, sr2, σ1', σ2'), (σpp, s)),
+          '(σl1, sr1, (σf1, σ1, (σpp1, s1, x1)), (σf2, σ2, (σpp2, s2, x2)))
+          '(σf, (σl2, sr2, σ1', σ2'), (σpp, s, x)),
            ∃ sp,
-           σ1 = σ1' ∧ σ2 = σ2' ∧ INV sp s1 s2 s sr1 sr2 ∧
-          (( sp = SPNone ∧
+           σ1 = σ1' ∧ σ2 = σ2' ∧ INV sp s1 s2 s x1 x2 sr1 sr2 ∧ ✓ x ∧
+          (* Here we have an ≡ instead of a ~~> since we know that the
+          resources in the spec must be up to date because the last
+          interaction was with the environment *)
+          (( sp = SPNone ∧ x ≡ x1 ⋅ x2 ∧
               σl1 = MLFNone ∧ σf = SMFilter
             ∧ σpp1 = PPOutside ∧ σpp2 = PPOutside ∧ σpp = PPOutside
             ∧ σf1 = SMFilter ∧ σf2 = SMFilter
             ∧ σl2 = MLFNone)
-           ∨ (sp = SPLeft ∧
+           ∨ (sp = SPLeft ∧ x ~~> x1 ⋅ x2 ∧
               ((∃ e, σl2 = MLFRecvL e ∧ σf1 = SMProgRecv (Incoming, e))
                ∨ (σl2 = MLFLeft ∧ σf1 = SMProg))
             ∧ σpp1 = PPInside ∧ σpp2 = PPOutside ∧ σpp = PPInside
             ∧ σf = SMProg ∧ σf2 = SMFilter
             ∧ σl1 = MLFLeft)
-           ∨ (sp = SPRight ∧
+           ∨ (sp = SPRight ∧ x ~~> x1 ⋅ x2 ∧
               ((∃ e, σl2 = MLFRecvR e ∧ σf2 = SMProgRecv (Incoming, e))
                ∨ (σl2 = MLFRight ∧ σf2 = SMProg))
             ∧ σpp1 = PPOutside ∧ σpp2 = PPInside ∧ σpp = PPInside
             ∧ σf = SMProg ∧ σf1 = SMFilter
             ∧ σl1 = MLFRight) )). }
       { split!. } { done. }
-      move => {}n _ /= Hloop {Hinv}.
-      move => [[[σl1 {}sr1] [[σf1 {}σ1] [σpp1 {}s1]]] [[σf2 {}σ2] [σpp2 {}s2]]].
-      move => [[σf [[[σl2 {}sr2] σ1'] σ2']] [σpp {}s]] ?. destruct_all?; simplify_eq.
-      - tstep_i => ? p' ???.
+      move => {}n _ /= Hloop {Hinv Hequiv Hvalid}.
+      move => [[[σl1 {}sr1] [[σf1 {}σ1] [[σpp1 {}s1] {}x1]]] [[σf2 {}σ2] [[σpp2 {}s2] {}x2]]].
+      move => [[σf [[[σl2 {}sr2] σ1'] σ2']] [[σpp {}s] {}x]] ?. destruct_all?; simplify_eq.
+      - revert select (✓ x) => Hvalid. revert select (x ≡ _) => Hequiv.
+        move: (Hvalid) => Hvalid2. rewrite Hequiv in Hvalid2.
+        tstep_i => ? p' ???.
         tstep_s. split!.
-        tstep_s. apply pp_to_all_forall => ri Hi.
+        tstep_s. apply pp_to_all_forall => ri xi Hi.
         destruct p' => /=. 3: naive_solver.
         + tstep_i => ??. simplify_eq.
-          tstep_i. move: ri Hi. apply pp_to_all_forall.
+          tstep_i. move: ri xi Hi. apply pp_to_all_forall.
+          apply: pp_to_all_mono_res; [done..|].
           apply: pp_to_all_mono; [by apply: HN2L|].
-          move => [[??]?] /= Hcont. apply: pp_to_ex_mono; [done|].
-          move => [[??]?] /= *. destruct_all?; simplify_eq.
+          move => [[??]?] ? /= Hcont ? ? Hequiv2. apply: pp_to_ex_mono; [done|].
+          move => [[??]?] ? /= *. destruct_all?; simplify_eq.
           tstep_s.
           split!; [done..|] => /=.
-          apply: Hloop; [done|]. by split!.
+          apply: Hloop; [done|]. split!. by rewrite Hequiv2.
         + tstep_i => ??. simplify_eq.
-          tstep_i. move: ri Hi. apply pp_to_all_forall.
+          tstep_i. move: ri xi Hi. apply pp_to_all_forall.
+          apply: pp_to_all_mono_res; [done..|].
           apply: pp_to_all_mono; [by apply: HN2R|].
-          move => [[??]?] /= Hcont. apply: pp_to_ex_mono; [done|].
-          move => [[??]?] /= *. destruct_all?; simplify_eq.
+          move => [[??]?] ? /= Hcont ? ? Hequiv2. apply: pp_to_ex_mono; [done|].
+          move => [[??]?] ? /= *. destruct_all?; simplify_eq.
           tstep_s.
           split!; [done..|] => /=.
-          apply: Hloop; [done|]. by split!.
+          apply: Hloop; [done|]. split!. by rewrite Hequiv2.
       - tstep_both.
         apply steps_impl_step_end => κ Pσ2 ?. case_match; intros; simplify_eq.
         + tstep_s. eexists (Some (Incoming, _)). split!.
@@ -393,29 +576,31 @@ Section prepost.
           apply: Hloop; [done|]. by split!.
         }
         tend. have [σ' Hσ'] := vis_no_all _ _ _ ltac:(done). eexists σ'. split; [naive_solver|].
-        tstep_i. apply pp_to_all_forall => ri Hi p' sr1' e' HR1 Hri.
+        tstep_i. apply pp_to_all_forall => ri xi Hi p' sr1' e' HR1 Hri.
+        have ?:= cmra_update_valid _ _ ltac:(done) ltac:(done).
         destruct p' => /=. 1: naive_solver.
         + tstep_i => ??; simplify_eq.
           tstep_i.
-          move: ri Hi sr1' e' Hri HR1. apply: pp_to_all_forall_2.
-          apply: pp_to_all_mono; [ by apply: HL2R|].
-          move => [[??]?] /= Hcont ????.
+          move: ri xi Hi sr1' e' Hri HR1. apply: pp_to_all_forall_2.
+          apply: pp_to_all_mono; [by apply: HL2R|].
+          move => [[??]?] ? /= Hcont ????.
           apply: pp_to_ex_mono; [ by apply: Hcont|].
-          move => [[??]?] /=?. destruct_all?; simplify_eq.
+          move => [[??]?] ? /=?. destruct_all?; simplify_eq.
           tstep_s. eexists (Some (Outgoing, _)). split!; [done|].
           destruct e; simplify_eq/=.
           apply: steps_spec_step_end; [done|] => ??.
-          apply: Hloop; [done|]. split!; [naive_solver|done..].
-        + move: ri Hi sr1' e' Hri HR1. apply: pp_to_all_forall_2.
+          apply: Hloop; [done|]. split!; [naive_solver|done..|by etrans].
+        + move: ri xi Hi sr1' e' Hri HR1. apply: pp_to_all_forall_2.
           apply: pp_to_all_mono; [by apply: HL2N|].
-          move => [[??]?] /= Hcont ????.
+          move => [[??]?] ? /= Hcont ????.
           have {}Hcont := Hcont _ _ ltac:(done) ltac:(done). destruct_all?.
           destruct e; simplify_eq/=.
           tstep_s. eexists (Some (Outgoing, _)). split!; [done|].
           apply: steps_spec_step_end; [done|] => ??.
           tstep_s.
+          apply: pp_to_ex_mono_res; [done..|].
           apply: pp_to_ex_mono; [done|].
-          move => [[??]?] /= *. destruct_all?; simplify_eq. split!.
+          move => [[??]?] ? /= ????. destruct_all?; simplify_eq. split!.
           apply: Hloop; [done|]. split!; [naive_solver|done..].
       - tstep_both.
         apply steps_impl_step_end => κ Pσ2 ?. case_match; intros; simplify_eq.
@@ -432,29 +617,31 @@ Section prepost.
           apply: Hloop; [done|]. by split!.
         }
         tend. have [σ' Hσ'] := vis_no_all _ _ _ ltac:(done). eexists σ'. split; [naive_solver|].
-        tstep_i. apply pp_to_all_forall => ri Hi p' sr1' e' HR1 Hri.
+        tstep_i. apply pp_to_all_forall => ri xi Hi p' sr1' e' HR1 Hri.
+        have ?:= cmra_update_valid _ _ ltac:(done) ltac:(done).
         destruct p' => /=. 2: naive_solver.
         + tstep_i => ??; simplify_eq.
           tstep_i.
-          move: ri Hi sr1' e' Hri HR1. apply: pp_to_all_forall_2.
-          apply: pp_to_all_mono; [ by apply: HR2L|].
-          move => [[??]?] /= Hcont ????.
+          move: ri xi Hi sr1' e' Hri HR1. apply: pp_to_all_forall_2.
+          apply: pp_to_all_mono; [by apply: HR2L|].
+          move => [[??]?] ? /= Hcont ????.
           apply: pp_to_ex_mono; [ by apply: Hcont|].
-          move => [[??]?] /= *. destruct_all?; simplify_eq.
+          move => [[??]?] ? /=?. destruct_all?; simplify_eq.
           tstep_s. eexists (Some (Outgoing, _)). split!; [done|].
           destruct e; simplify_eq/=.
           apply: steps_spec_step_end; [done|] => ??.
-          apply: Hloop; [done|]. split!; [naive_solver|done..].
-        + move: ri Hi sr1' e' Hri HR1. apply: pp_to_all_forall_2.
+          apply: Hloop; [done|]. split!; [naive_solver|done..|by etrans].
+        + move: ri xi Hi sr1' e' Hri HR1. apply: pp_to_all_forall_2.
           apply: pp_to_all_mono; [by apply: HR2N|].
-          move => [[??]?] /= Hcont ????.
+          move => [[??]?] ? /= Hcont ????.
           have {}Hcont := Hcont _ _ ltac:(done) ltac:(done). destruct_all?.
           destruct e; simplify_eq/=.
           tstep_s. eexists (Some (Outgoing, _)). split!; [done|].
           apply: steps_spec_step_end; [done|] => ??.
           tstep_s.
+          apply: pp_to_ex_mono_res; [done..|].
           apply: pp_to_ex_mono; [done|].
-          move => [[??]?] /= *. destruct_all?; simplify_eq. split!.
+          move => [[??]?] ? /= ????. destruct_all?; simplify_eq. split!.
           apply: Hloop; [done|]. split!; [naive_solver|done..].
     Qed.
 End prepost.
